formal/fstar/ocaml-output/XML_Namespaces.ml
@@ -1,0 +1,212 @@
+open Prims
+let xml_ns_uri : Prims.string= "http://www.w3.org/XML/1998/namespace"
+let xmlns_ns_uri : Prims.string= "http://www.w3.org/2000/xmlns/"
+type qname_split =
+  | QSimple of Prims.string 
+  | QPrefixed of Prims.string * Prims.string 
+  | QMalformed 
+let uu___is_QSimple (projectee : qname_split) : Prims.bool=
+  match projectee with | QSimple local -> true | uu___ -> false
+let __proj__QSimple__item__local (projectee : qname_split) : Prims.string=
+  match projectee with | QSimple local -> local
+let uu___is_QPrefixed (projectee : qname_split) : Prims.bool=
+  match projectee with | QPrefixed (prefix, local) -> true | uu___ -> false
+let __proj__QPrefixed__item__prefix (projectee : qname_split) : Prims.string=
+  match projectee with | QPrefixed (prefix, local) -> prefix
+let __proj__QPrefixed__item__local (projectee : qname_split) : Prims.string=
+  match projectee with | QPrefixed (prefix, local) -> local
+let uu___is_QMalformed (projectee : qname_split) : Prims.bool=
+  match projectee with | QMalformed -> true | uu___ -> false
+let rec find_colon_positions (s : Prims.string) (pos : Prims.nat)
+  (limit : Prims.nat) (fuel : Prims.nat) (acc : Prims.nat Prims.list) :
+  Prims.nat Prims.list=
+  if fuel = Prims.int_zero
+  then FStar_List_Tot_Base.rev acc
+  else
+    if pos >= limit
+    then FStar_List_Tot_Base.rev acc
+    else
+      (let c = Parser_FastString.fs_byte_index s pos in
+       if c = 58
+       then
+         find_colon_positions s (pos + Prims.int_one) limit
+           (fuel - Prims.int_one) (pos :: acc)
+       else
+         find_colon_positions s (pos + Prims.int_one) limit
+           (fuel - Prims.int_one) acc)
+let split_qname (s : Prims.string) : qname_split=
+  let len = Parser_FastString.fs_byte_length s in
+  match find_colon_positions s Prims.int_zero len len [] with
+  | [] -> QSimple s
+  | i::[] ->
+      if (i = Prims.int_zero) || ((i + Prims.int_one) >= len)
+      then QMalformed
+      else
+        QPrefixed
+          ((Parser_FastString.fs_byte_sub s Prims.int_zero i),
+            (Parser_FastString.fs_byte_sub s (i + Prims.int_one)
+               (len - (i + Prims.int_one))))
+  | uu___ -> QMalformed
+type ns_scope =
+  (Prims.string * Prims.string FStar_Pervasives_Native.option) Prims.list
+let initial_scope : ns_scope=
+  [("xml", (FStar_Pervasives_Native.Some xml_ns_uri))]
+let rec lookup_prefix (scope : ns_scope) (prefix : Prims.string) :
+  Prims.string FStar_Pervasives_Native.option=
+  match scope with
+  | [] -> FStar_Pervasives_Native.None
+  | (p, u)::rest -> if p = prefix then u else lookup_prefix rest prefix
+let rec apply_declarations (version : Prims.string) (scope : ns_scope)
+  (attrs : Parser_XML.xml_attribute Prims.list) :
+  ns_scope FStar_Pervasives_Native.option=
+  match attrs with
+  | [] -> FStar_Pervasives_Native.Some scope
+  | a::rest ->
+      (match split_qname a.Parser_XML.attr_name with
+       | QSimple "xmlns" ->
+           let v = a.Parser_XML.attr_value in
+           if (v = xml_ns_uri) || (v = xmlns_ns_uri)
+           then FStar_Pervasives_Native.None
+           else
+             (let entry =
+                if v = ""
+                then ("", FStar_Pervasives_Native.None)
+                else ("", (FStar_Pervasives_Native.Some v)) in
+              match apply_declarations version scope rest with
+              | FStar_Pervasives_Native.None -> FStar_Pervasives_Native.None
+              | FStar_Pervasives_Native.Some sc ->
+                  FStar_Pervasives_Native.Some (entry :: sc))
+       | QPrefixed ("xmlns", local) ->
+           let v = a.Parser_XML.attr_value in
+           if local = "xmlns"
+           then FStar_Pervasives_Native.None
+           else
+             if (local = "xml") && (v <> xml_ns_uri)
+             then FStar_Pervasives_Native.None
+             else
+               if (local <> "xml") && (v = xml_ns_uri)
+               then FStar_Pervasives_Native.None
+               else
+                 if v = xmlns_ns_uri
+                 then FStar_Pervasives_Native.None
+                 else
+                   if (v = "") && (version <> "1.1")
+                   then FStar_Pervasives_Native.None
+                   else
+                     (let entry =
+                        if v = ""
+                        then (local, FStar_Pervasives_Native.None)
+                        else (local, (FStar_Pervasives_Native.Some v)) in
+                      match apply_declarations version scope rest with
+                      | FStar_Pervasives_Native.None ->
+                          FStar_Pervasives_Native.None
+                      | FStar_Pervasives_Native.Some sc ->
+                          FStar_Pervasives_Native.Some (entry :: sc))
+       | uu___ -> apply_declarations version scope rest)
+let rec all_attr_names_wellformed
+  (attrs : Parser_XML.xml_attribute Prims.list) : Prims.bool=
+  match attrs with
+  | [] -> true
+  | a::rest ->
+      (match split_qname a.Parser_XML.attr_name with
+       | QMalformed -> false
+       | uu___ -> all_attr_names_wellformed rest)
+let tag_prefix_bound (scope : ns_scope) (qs : qname_split) : Prims.bool=
+  match qs with
+  | QSimple uu___ -> true
+  | QPrefixed (pfx, uu___) ->
+      (match lookup_prefix scope pfx with
+       | FStar_Pervasives_Native.Some uu___1 -> true
+       | FStar_Pervasives_Native.None -> false)
+  | QMalformed -> false
+let rec attrs_prefixes_bound (scope : ns_scope)
+  (attrs : Parser_XML.xml_attribute Prims.list) : Prims.bool=
+  match attrs with
+  | [] -> true
+  | a::rest ->
+      (match split_qname a.Parser_XML.attr_name with
+       | QSimple "xmlns" -> attrs_prefixes_bound scope rest
+       | QPrefixed ("xmlns", uu___) -> attrs_prefixes_bound scope rest
+       | QSimple uu___ -> attrs_prefixes_bound scope rest
+       | QPrefixed (pfx, uu___) ->
+           (match lookup_prefix scope pfx with
+            | FStar_Pervasives_Native.Some uu___1 ->
+                attrs_prefixes_bound scope rest
+            | FStar_Pervasives_Native.None -> false)
+       | QMalformed -> false)
+let expand_attr_key (scope : ns_scope) (a : Parser_XML.xml_attribute) :
+  (Prims.string FStar_Pervasives_Native.option * Prims.string)
+    FStar_Pervasives_Native.option=
+  match split_qname a.Parser_XML.attr_name with
+  | QSimple "xmlns" -> FStar_Pervasives_Native.None
+  | QPrefixed ("xmlns", uu___) -> FStar_Pervasives_Native.None
+  | QSimple name ->
+      FStar_Pervasives_Native.Some (FStar_Pervasives_Native.None, name)
+  | QPrefixed (pfx, local) ->
+      FStar_Pervasives_Native.Some ((lookup_prefix scope pfx), local)
+  | QMalformed -> FStar_Pervasives_Native.None
+let rec expand_attr_keys (scope : ns_scope)
+  (attrs : Parser_XML.xml_attribute Prims.list) :
+  (Prims.string FStar_Pervasives_Native.option * Prims.string) Prims.list=
+  match attrs with
+  | [] -> []
+  | a::rest ->
+      (match expand_attr_key scope a with
+       | FStar_Pervasives_Native.Some k -> k :: (expand_attr_keys scope rest)
+       | FStar_Pervasives_Native.None -> expand_attr_keys scope rest)
+let rec mem_key
+  (k : (Prims.string FStar_Pervasives_Native.option * Prims.string))
+  (ks :
+    (Prims.string FStar_Pervasives_Native.option * Prims.string) Prims.list)
+  : Prims.bool=
+  match ks with
+  | [] -> false
+  | k2::rest -> if k = k2 then true else mem_key k rest
+let rec keys_unique
+  (ks :
+    (Prims.string FStar_Pervasives_Native.option * Prims.string) Prims.list)
+  : Prims.bool=
+  match ks with
+  | [] -> true
+  | k::rest -> if mem_key k rest then false else keys_unique rest
+let attrs_unique_expanded (scope : ns_scope)
+  (attrs : Parser_XML.xml_attribute Prims.list) : Prims.bool=
+  keys_unique (expand_attr_keys scope attrs)
+let rec check_element (version : Prims.string) (scope : ns_scope)
+  (node : Parser_XML.xml_node) : Prims.bool=
+  match node with
+  | Parser_XML.XElement (tag, attrs, children) ->
+      (match split_qname tag with
+       | QMalformed -> false
+       | tag_split ->
+           if Prims.op_Negation (all_attr_names_wellformed attrs)
+           then false
+           else
+             (match apply_declarations version scope attrs with
+              | FStar_Pervasives_Native.None -> false
+              | FStar_Pervasives_Native.Some new_scope ->
+                  if Prims.op_Negation (tag_prefix_bound new_scope tag_split)
+                  then false
+                  else
+                    if
+                      Prims.op_Negation
+                        (attrs_prefixes_bound new_scope attrs)
+                    then false
+                    else
+                      if
+                        Prims.op_Negation
+                          (attrs_unique_expanded new_scope attrs)
+                      then false
+                      else check_children version new_scope children))
+  | uu___ -> true
+and check_children (version : Prims.string) (scope : ns_scope)
+  (nodes : Parser_XML.xml_node Prims.list) : Prims.bool=
+  match nodes with
+  | [] -> true
+  | hd::tl ->
+      if check_element version scope hd
+      then check_children version scope tl
+      else false
+let is_namespace_wellformed (version : Prims.string)
+  (root : Parser_XML.xml_node) : Prims.bool=
+  check_element version initial_scope root
